nondeterministic_dataflow/Cset_Setup.thy
@@ -1,0 +1,66 @@
+text \<open>cset setup\<close>
+
+theory Cset_Setup
+
+imports
+  "HOL-Library.Countable_Set_Type"
+begin
+
+section \<open>cset Syntax\<close>
+syntax
+  "_insert_fset"     :: "args => 'a cset"  ("{|(_)|}")
+
+notation cempty ("{||}")
+
+translations
+  "{|x, xs|}" == "CONST cinsert x {|xs|}"
+  "{|x|}"     == "CONST csingle x"
+
+abbreviation cmember :: "'a \<Rightarrow> 'a cset \<Rightarrow> bool" (infix "|\<in>|" 50) where
+  "x |\<in>| X \<equiv> cin x X"
+
+section \<open>cset lifts\<close>
+context includes cset.lifting begin
+lift_definition natcUNIV :: "nat cset" is UNIV by auto
+lift_definition cproduct :: "'a cset \<Rightarrow> 'b cset \<Rightarrow> ('a \<times> 'b) cset" is "(\<times>)" by auto
+lift_definition cfilter :: "('a \<Rightarrow> bool) \<Rightarrow> 'a cset \<Rightarrow> 'a cset" is Set.filter by (simp add: Set.filter_def)
+lift_definition cUNIV :: "('m :: countable) cset" is UNIV by auto
+
+end
+
+declare cBall.rep_eq[simp] cinsert.rep_eq[simp] bot_cset.rep_eq[simp] sup_cset.rep_eq[simp] cimage.rep_eq[simp] cUnion.rep_eq[simp] rel_cset.rep_eq[simp]
+  cfilter.rep_eq[simp]
+
+lemma cfilter_eq[simp]:
+  "cfilter P A = B \<longleftrightarrow>
+   Set.filter P (cset.rcset A) = (cset.rcset B)"
+  by (auto simp add: cin.rep_eq)
+
+lemma cin_cfilter[simp]:
+  "x |\<in>| cfilter P A \<longleftrightarrow> x |\<in>| A \<and> P x"
+  by (metis cfilter.rep_eq cin.rep_eq member_filter)
+
+
+lemma cin_cimage_cfilter[simp]:
+  "x |\<in>| cimage f (cfilter P A) \<longleftrightarrow> (\<exists> y. y |\<in>| A \<and> P y \<and> x = f y)"
+  by auto
+
+lemma cUnion_cempty[simp]:
+  "cUnion {||} = {||}"
+  using cUN_empty by auto
+
+lemma cfilter_cempty[simp]:
+  "cfilter P {||} = {||}"
+  by auto
+
+lemma cfilter_cfilter[simp]:
+  "cfilter P (cfilter P S) = cfilter P S"
+  by force
+
+lemma cUnion_cinsert[simp]:
+  "cUnion (cinsert x A) = cUn x (cUnion A)"
+  apply (subst (3 8) cset.map_id[symmetric])
+  apply (metis cUN_cinsert eq_id_iff)
+  done
+
+end
